Definition of Validity

theories/Substitution/Properties.v
@@ -1,6 +1,6 @@
 From LogRel.AutoSubst Require Import core unscoped Ast Extra.
-From LogRel Require Import Utils BasicAst Notations Context NormalForms UntypedValues Weakening GenericTyping LogicalRelation DeclarativeInstance Validity.
-From LogRel.LogicalRelation Require Import Irrelevance Escape Reflexivity Weakening Neutral Induction.
+From LogRel Require Import Utils BasicAst Notations LContexts Context NormalForms Weakening GenericTyping Monad LogicalRelation Validity.
+From LogRel.LogicalRelation Require Import Irrelevance Escape Reflexivity Weakening Neutral Induction Monotonicity.
 From LogRel.Substitution Require Import Irrelevance.
 
 Set Universe Polymorphism.
@@ -9,225 +9,222 @@ Section Properties.
 Context `{GenericTypingProperties}.
 
 
-Lemma wellformedSubst {Γ σ Δ} (VΓ : [||-v Γ]) (wfΔ : [|- Δ]) :
-  [Δ ||-v σ : Γ | VΓ| wfΔ] -> [Δ |-s σ : Γ ].
+Lemma wellformedSubst {wl Γ σ Δ} (VΓ : [||-v Γ]< wl >) (wfΔ : [|- Δ]< wl >) :
+  [Δ ||-v σ : Γ | VΓ| wfΔ]< wl > -> [Δ |-s σ : Γ ]< wl >.
 Proof.
   revert σ; pattern Γ, VΓ; apply validity_rect; clear Γ VΓ.
   - intros. apply well_sempty.
   - intros * ih σ [tl hd].
     eapply well_scons.
     + now apply ih.
-    + now escape.
+    + now Wescape.
 Qed.
 
-Lemma wellformedSubstEq {Γ σ σ' Δ} (VΓ : [||-v Γ]) (wfΔ : [|- Δ]) (Vσ : [Δ ||-v σ : Γ | VΓ | wfΔ]) :
-  [Δ ||-v σ ≅ σ' : Γ | VΓ | wfΔ | Vσ] -> [Δ |-s σ ≅ σ' : Γ].
+Lemma wellformedSubstEq {wl Γ σ σ' Δ} (VΓ : [||-v Γ]< wl >) (wfΔ : [|- Δ]< wl >) (Vσ : [Δ ||-v σ : Γ | VΓ | wfΔ]< wl >) :
+  [Δ ||-v σ ≅ σ' : Γ | VΓ | wfΔ | Vσ]< wl > -> [Δ |-s σ ≅ σ' : Γ]< wl >.
 Proof.
   revert σ σ' Vσ; pattern Γ, VΓ; apply validity_rect; clear Γ VΓ.
   - intros. apply conv_sempty.
   - intros * ih ??? [tl hd]. apply conv_scons.
     + now eapply ih.
-    + now escape.
+    + now Wescape.
 Qed.
 
-Lemma consSubstS {Γ σ t l A Δ} (VΓ : [||-v Γ]) (wfΔ : [|- Δ])
-  (Vσ : [Δ ||-v σ : Γ | VΓ | wfΔ]) (VA : [Γ ||-v<l> A | VΓ])
-  (Vt : [ Δ ||-<l> t : A[σ] | validTy VA wfΔ Vσ]) :
-  [Δ ||-v (t .: σ) : Γ ,, A | validSnoc VΓ VA | wfΔ].
+Lemma consSubstS {wl Γ σ t l A Δ} (VΓ : [||-v Γ]< wl >) (wfΔ : [|- Δ]< wl >)
+  (Vσ : [Δ ||-v σ : Γ | VΓ | wfΔ]< wl >) (VA : [Γ ||-v<l> A | VΓ]< wl >)
+  (Vt : W[ Δ ||-<l> t : A[σ] | validTy VA wfΔ Vσ]< wl >) :
+  [Δ ||-v (t .: σ) : Γ ,, A | validSnoc VΓ VA | wfΔ]< wl >.
 Proof.  unshelve econstructor; eassumption. Defined.
 
-Lemma consValid {Γ Δ σ a A l} {VΓ : [||-v Γ]} {wfΔ : [|- Δ]}
-  (Vσ : [Δ ||-v σ : Γ | VΓ | wfΔ])
-  {VA : [Γ ||-v<l> A| VΓ]}
-  (Va : [Γ ||-v<l> a : A | VΓ | VA])
-  (VΓA := validSnoc VΓ VA) :
-  [Δ ||-v (a[σ] .: σ) : Γ,, A | VΓA | wfΔ].
-Proof.
-  unshelve eapply consSubstS; tea; now eapply validTm.
-Qed.
 
-
-Lemma consSubstSEq {Γ σ σ' t l A Δ} (VΓ : [||-v Γ]) (wfΔ : [|- Δ])
-  (Vσ : [Δ ||-v σ : Γ | VΓ | wfΔ])
-  (Vσσ' : [Δ ||-v σ ≅ σ' : Γ | VΓ | wfΔ | Vσ])
-  (VA : [Γ ||-v<l> A | VΓ])
-  (Vt : [Δ ||-<l> t : A[σ] | validTy VA wfΔ Vσ]) :
-  [Δ ||-v (t .: σ) ≅  (t .: σ') : Γ ,, A | validSnoc VΓ VA | wfΔ | consSubstS VΓ wfΔ Vσ VA Vt].
+Lemma consSubstSEq {wl Γ σ σ' t l A Δ} (VΓ : [||-v Γ]< wl >) (wfΔ : [|- Δ]< wl >)
+  (Vσ : [Δ ||-v σ : Γ | VΓ | wfΔ]< wl >)
+  (Vσσ' : [Δ ||-v σ ≅ σ' : Γ | VΓ | wfΔ | Vσ]< wl >)
+  (VA : [Γ ||-v<l> A | VΓ]< wl >)
+  (Vt : W[Δ ||-<l> t : A[σ] | validTy VA wfΔ Vσ]< wl >) :
+  [Δ ||-v (t .: σ) ≅  (t .: σ') : Γ ,, A | validSnoc VΓ VA | wfΔ | consSubstS VΓ wfΔ Vσ VA Vt]< wl >.
 Proof.
   unshelve econstructor.
   1: eassumption.
-  eapply LRTmEqRefl; [apply (validTy VA wfΔ)| exact Vt].
+  eapply WreflLRTmEq ; exact Vt.
 Qed.
 
-Lemma consSubstSEq' {Γ σ σ' t u l A Δ} (VΓ : [||-v Γ]) (wfΔ : [|- Δ])
-  (Vσ : [Δ ||-v σ : Γ | VΓ | wfΔ])
-  (Vσσ' : [Δ ||-v σ ≅ σ' : Γ | VΓ | wfΔ | Vσ])
-  (VA : [Γ ||-v<l> A | VΓ])
-  (Vt : [Δ ||-<l> t : A[σ] | validTy VA wfΔ Vσ])
-  (Vtu : [Δ ||-<l> t ≅ u : A[σ] | validTy VA wfΔ Vσ]) :
-  [Δ ||-v (t .: σ) ≅  (u .: σ') : Γ ,, A | validSnoc VΓ VA | wfΔ | consSubstS VΓ wfΔ Vσ VA Vt].
+Lemma consSubstSEq' {wl Γ σ σ' t u l A Δ} (VΓ : [||-v Γ]< wl >) (wfΔ : [|- Δ]< wl >)
+  (Vσ : [Δ ||-v σ : Γ | VΓ | wfΔ]< wl >)
+  (Vσσ' : [Δ ||-v σ ≅ σ' : Γ | VΓ | wfΔ | Vσ]< wl >)
+  (VA : [Γ ||-v<l> A | VΓ]< wl >)
+  (Vt : W[Δ ||-<l> t : A[σ] | validTy VA wfΔ Vσ]< wl >)
+  (Vtu : W[Δ ||-<l> t ≅ u : A[σ] | validTy VA wfΔ Vσ]< wl >) :
+  [Δ ||-v (t .: σ) ≅  (u .: σ') : Γ ,, A | validSnoc VΓ VA | wfΔ | consSubstS VΓ wfΔ Vσ VA Vt]< wl >.
 Proof.
   unshelve econstructor; tea.
 Qed.  
 
 
-Lemma consSubstSvalid {Γ σ t l A Δ} (VΓ : [||-v Γ]) (wfΔ : [|- Δ])
-  (Vσ : [Δ ||-v σ : Γ | VΓ | wfΔ]) (VA : [Γ ||-v<l> A | VΓ])
-  (Vt : [ Γ ||-v<l> t : A | VΓ | VA]) :
-  [Δ ||-v (t[σ] .: σ) : Γ ,, A | validSnoc VΓ VA | wfΔ].
+Lemma consSubstSvalid {wl Γ σ t l A Δ} {VΓ : [||-v Γ]< wl >} {wfΔ : [|- Δ]< wl >}
+  (Vσ : [Δ ||-v σ : Γ | VΓ | wfΔ]< wl >) {VA : [Γ ||-v<l> A | VΓ]< wl >}
+  (Vt : [ Γ ||-v<l> t : A | VΓ | VA]< wl >) :
+  [Δ ||-v (t[σ] .: σ) : Γ ,, A | validSnoc VΓ VA | wfΔ]< wl >.
 Proof. unshelve eapply consSubstS; tea; now eapply validTm. Defined.
 
 Set Printing Primitive Projection Parameters.
 
-Lemma consSubstSEqvalid {Γ σ σ' t l A Δ} (VΓ : [||-v Γ]) (wfΔ : [|- Δ])
-  (Vσ : [Δ ||-v σ : Γ | VΓ | wfΔ]) 
-  (Vσ' : [Δ ||-v σ' : Γ | VΓ | wfΔ]) 
-  (Vσσ' : [Δ ||-v σ ≅ σ' : Γ | VΓ | wfΔ | Vσ])
-  (VA : [Γ ||-v<l> A | VΓ])
-  (Vt : [Γ ||-v<l> t : A | VΓ | VA]) :
-  [Δ ||-v (t[σ] .: σ) ≅  (t[σ'] .: σ') : Γ ,, A | validSnoc VΓ VA | wfΔ | consSubstSvalid VΓ wfΔ Vσ VA Vt].
+Lemma consSubstSEqvalid {wl Γ σ σ' t l A Δ} {VΓ : [||-v Γ]< wl >} {wfΔ : [|- Δ]< wl >}
+  (Vσ : [Δ ||-v σ : Γ | VΓ | wfΔ]< wl >)
+  (Vσ' : [Δ ||-v σ' : Γ | VΓ | wfΔ]< wl >) 
+  (Vσσ' : [Δ ||-v σ ≅ σ' : Γ | VΓ | wfΔ | Vσ]< wl >)
+  {VA : [Γ ||-v<l> A | VΓ]< wl >}
+  (Vt : [Γ ||-v<l> t : A | VΓ | VA]< wl >) :
+  [Δ ||-v (t[σ] .: σ) ≅  (t[σ'] .: σ') : Γ ,, A | validSnoc VΓ VA | wfΔ | consSubstSvalid Vσ Vt]< wl >.
 Proof.
   unshelve econstructor; intros; tea.
   now apply validTmExt.
 Qed.
 
-Lemma wkSubstS {Γ} (VΓ : [||-v Γ]) : 
-  forall {σ  Δ Δ'}  (wfΔ : [|- Δ]) (wfΔ' : [|- Δ']) (ρ : Δ' ≤ Δ),
-  [Δ ||-v σ : Γ | VΓ | wfΔ] -> [Δ' ||-v σ ⟨ ρ ⟩ : Γ | VΓ | wfΔ'].
+Lemma wkSubstS {wl Γ} (VΓ : [||-v Γ]< wl >) : 
+  forall {σ  Δ Δ'}  (wfΔ : [|- Δ]< wl >) (wfΔ' : [|- Δ']< wl >) (ρ : Δ' ≤ Δ),
+  [Δ ||-v σ : Γ | VΓ | wfΔ]< wl > -> [Δ' ||-v σ ⟨ ρ ⟩ : Γ | VΓ | wfΔ']< wl >.
 Proof.
   pattern Γ, VΓ ; apply validity_rect; clear Γ VΓ.
   - constructor.
   - intros * ih * [tl hd]. unshelve econstructor.
     + eapply ih; eassumption.
-    + eapply LRTmRedIrrelevant'.
-      2: eapply (wkTerm _ wfΔ') ; exact hd.
+    + eapply WLRTmRedIrrelevant'.
+      2: eapply (WwkTerm _ wfΔ') ; exact hd.
       now asimpl.
 Defined.
 
 
-Lemma wkSubstSEq {Γ} (VΓ : [||-v Γ]) :
-  forall {σ σ' Δ Δ'}  (wfΔ : [|- Δ]) (wfΔ' : [|- Δ']) (ρ : Δ' ≤ Δ)
-  (Vσ : [Δ ||-v σ : Γ | VΓ | wfΔ]),
-  [Δ  ||-v σ ≅ σ' : Γ | VΓ | wfΔ | Vσ] ->
-  [Δ' ||-v σ ⟨ ρ ⟩ ≅ σ' ⟨ ρ ⟩ : Γ | VΓ | wfΔ' | wkSubstS VΓ wfΔ wfΔ' ρ Vσ].
+Lemma wkSubstSEq {wl Γ} (VΓ : [||-v Γ]< wl >) :
+  forall {σ σ' Δ Δ'}  (wfΔ : [|- Δ]< wl >) (wfΔ' : [|- Δ']< wl >) (ρ : Δ' ≤ Δ)
+  (Vσ : [Δ ||-v σ : Γ | VΓ | wfΔ]< wl >),
+  [Δ  ||-v σ ≅ σ' : Γ | VΓ | wfΔ | Vσ]< wl > ->
+  [Δ' ||-v σ ⟨ ρ ⟩ ≅ σ' ⟨ ρ ⟩ : Γ | VΓ | wfΔ' | wkSubstS VΓ wfΔ wfΔ' ρ Vσ]< wl >.
 Proof.
   pattern Γ, VΓ; apply validity_rect; clear Γ VΓ.
   - constructor.
   - intros * ih * [tl hd]; unshelve econstructor.
     + eapply ih ; eassumption.
-    + eapply LRTmEqIrrelevant'.
-      2: eapply (wkTermEq _ wfΔ') ; exact hd.
+    + eapply WLRTmEqIrrelevant'.
+      2: eapply (WwkTermEq _ wfΔ') ; exact hd.
       now asimpl.
 Qed.
 
-Lemma wk1SubstS {Γ σ Δ F} (VΓ : [||-v Γ]) (wfΔ : [|- Δ]) (wfF : [Δ |- F]) :
-  [Δ ||-v σ : Γ | VΓ | wfΔ ] ->
-  [Δ ,, F ||-v σ ⟨ @wk1 Δ F ⟩ : Γ | VΓ | wfc_cons wfΔ wfF].
+Lemma wk1SubstS {wl Γ σ Δ F} (VΓ : [||-v Γ]< wl >) (wfΔ : [|- Δ]< wl >) (wfF : [Δ |- F]< wl >) :
+  [Δ ||-v σ : Γ | VΓ | wfΔ ]< wl > ->
+  [Δ ,, F ||-v σ ⟨ @wk1 Δ F ⟩ : Γ | VΓ | wfc_cons wfΔ wfF]< wl >.
 Proof. eapply wkSubstS. Defined.
 
-Lemma wk1SubstSEq {Γ σ σ' Δ F} (VΓ : [||-v Γ])
-  (wfΔ : [|- Δ]) (wfF : [Δ |- F])
-  (Vσ : [Δ ||-v σ : Γ | VΓ | wfΔ ]) :
-  [Δ ||-v σ ≅ σ' : Γ | VΓ | wfΔ | Vσ] ->
+Lemma wk1SubstSEq {wl Γ σ σ' Δ F} (VΓ : [||-v Γ]< wl >)
+  (wfΔ : [|- Δ]< wl >) (wfF : [Δ |- F]< wl >)
+  (Vσ : [Δ ||-v σ : Γ | VΓ | wfΔ ]< wl >) :
+  [Δ ||-v σ ≅ σ' : Γ | VΓ | wfΔ | Vσ]< wl > ->
   let ρ := @wk1 Δ F in
-  [Δ ,, F ||-v σ ⟨ ρ ⟩ ≅ σ' ⟨ ρ ⟩ : Γ | VΓ | wfc_cons wfΔ wfF | wk1SubstS VΓ wfΔ wfF Vσ].
+  [Δ ,, F ||-v σ ⟨ ρ ⟩ ≅ σ' ⟨ ρ ⟩ : Γ | VΓ | wfc_cons wfΔ wfF | wk1SubstS VΓ wfΔ wfF Vσ]< wl >.
 Proof.
   intro vσσ'. eapply wkSubstSEq ; eassumption.
 Qed.
 
-Lemma consWkSubstS {Γ F Δ Ξ σ a l VΓ wfΔ } VF
+Lemma consWkSubstS {wl Γ F Δ Ξ σ a l VΓ wfΔ } VF
   (ρ : Ξ ≤ Δ) wfΞ {RF}:
-  [Δ ||-v σ : Γ | VΓ | wfΔ] ->
-  [Ξ ||-<l> a : F[σ]⟨ρ⟩ | RF] ->
-  [Ξ ||-v (a .: σ⟨ρ⟩) : Γ,, F | validSnoc (l:=l) VΓ VF | wfΞ].
+  [Δ ||-v σ : Γ | VΓ | wfΔ]< wl > ->
+  W[Ξ ||-<l> a : F[σ]⟨ρ⟩ | RF]< wl > ->
+  [Ξ ||-v (a .: σ⟨ρ⟩) : Γ,, F | validSnoc (l:=l) VΓ VF | wfΞ]< wl >.
 Proof.
-  intros. unshelve eapply consSubstS.  2: irrelevance.
+  intros. unshelve eapply consSubstS.  2: Wirrelevance.
   now eapply wkSubstS.
 Qed.
 
+Lemma consWkSubstSEq' {wl Γ Δ Ξ A σ σ' a b l} {VΓ : [||-v Γ]< wl >} {wfΔ : [|- Δ]< wl >}
+  (VA : [Γ ||-v<l> A | VΓ]< wl >)
+  (Vσ : [Δ ||-v σ : Γ | VΓ | wfΔ]< wl >)
+  (Vσσ' : [Δ ||-v σ ≅ σ' : Γ | VΓ | wfΔ | Vσ]< wl >)
+  (ρ : Ξ ≤ Δ) wfΞ {RA}
+  (Ra : W[Ξ ||-<l> a : A[σ]⟨ρ⟩ | RA]< wl >)
+  (Rab : W[Ξ ||-<l> a ≅ b : A[σ]⟨ρ⟩ | RA]< wl >) 
+  (Vawkσ := consWkSubstS VA ρ wfΞ Vσ Ra) :
+  [Ξ ||-v (a .: σ⟨ρ⟩) ≅  (b .: σ'⟨ρ⟩) : Γ ,, A | validSnoc VΓ VA | wfΞ | Vawkσ]< wl >.
+Proof.
+  unshelve eapply consSubstSEq'.
+  - unshelve eapply irrelevanceSubstEq.
+    4: now eapply wkSubstSEq.
+    tea.
+  - Wirrelevance0; tea. now bsimpl.
+Qed.  
 
-Lemma liftSubstS {Γ σ Δ lF F} (VΓ : [||-v Γ]) (wfΔ : [|- Δ])
-  (VF : [Γ ||-v<lF> F | VΓ])
-  (Vσ : [Δ ||-v σ : Γ | VΓ | wfΔ ]) :
+
+Lemma liftSubstS {wl Γ σ Δ lF F} (VΓ : [||-v Γ]< wl >) (wfΔ : [|- Δ]< wl >)
+  (VF : [Γ ||-v<lF> F | VΓ]< wl >)
+  (Vσ : [Δ ||-v σ : Γ | VΓ | wfΔ ]< wl >) :
   let VΓF := validSnoc VΓ VF in
   let ρ := @wk1 Δ F[σ] in
-  let wfΔF := wfc_cons wfΔ (escape (validTy VF wfΔ Vσ)) in
-  [Δ ,, F[σ] ||-v (tRel 0 .: σ ⟨ ρ ⟩) : Γ ,, F | VΓF | wfΔF ].
+  let wfΔF := wfc_cons wfΔ (Wescape (validTy VF wfΔ Vσ)) in
+  [Δ ,, F[σ] ||-v (tRel 0 .: σ ⟨ ρ ⟩) : Γ ,, F | VΓF | wfΔF ]< wl >.
 Proof.
   intros; unshelve econstructor.
   - now eapply wk1SubstS.
-  - eapply var0; unfold ρ; [now bsimpl|].
-    now eapply escape, VF.
+  - eapply Wvar0 ; unfold ρ; [now bsimpl|].
+    now eapply Wescape, VF.
 Defined.
 
-Lemma liftSubstSrealign {Γ σ σ' Δ lF F} {VΓ : [||-v Γ]} {wfΔ : [|- Δ]}
-  (VF : [Γ ||-v<lF> F | VΓ])
-  {Vσ : [Δ ||-v σ : Γ | VΓ | wfΔ ]} :
+Lemma liftSubstSrealign {wl Γ σ σ' Δ lF F} {VΓ : [||-v Γ]< wl >} {wfΔ : [|- Δ]< wl >}
+  (VF : [Γ ||-v<lF> F | VΓ]< wl >)
+  {Vσ : [Δ ||-v σ : Γ | VΓ | wfΔ ]< wl >} :
   let VΓF := validSnoc VΓ VF in
   let ρ := @wk1 Δ F[σ]  in
-  let wfΔF := wfc_cons wfΔ (escape (validTy VF wfΔ Vσ)) in
-  [Δ ||-v σ ≅ σ' : Γ | VΓ | wfΔ | Vσ] ->
-  [Δ ||-v σ' : Γ | VΓ | wfΔ ] ->
-  [Δ ,, F[σ] ||-v (tRel 0 .: σ'⟨ρ⟩) : Γ ,, F | VΓF | wfΔF].
+  let wfΔF := wfc_cons wfΔ (Wescape (validTy VF wfΔ Vσ)) in
+  [Δ ||-v σ ≅ σ' : Γ | VΓ | wfΔ | Vσ]< wl > ->
+  [Δ ||-v σ' : Γ | VΓ | wfΔ ]< wl > ->
+  [Δ ,, F[σ] ||-v (tRel 0 .: σ'⟨ρ⟩) : Γ ,, F | VΓF | wfΔF]< wl >.
 Proof.
   intros; unshelve econstructor.
   + now eapply wk1SubstS.
   + cbn.
-    assert [Δ,, F[σ] |-[ ta ] tRel 0 : F[S >> (tRel 0 .: σ'⟨ρ⟩)]].
+    assert [Δ,, F[σ] |-[ ta ] tRel 0 : F[S >> (tRel 0 .: σ'⟨ρ⟩)]]< wl >.
     { replace F[_ >> _] with F[σ']⟨S⟩ by (unfold ρ; now bsimpl).
       eapply ty_conv. 1: apply (ty_var wfΔF (in_here _ _)).
       cbn; renToWk. eapply convty_wk; tea.
-      eapply escapeEq;  unshelve eapply validTyExt; cycle 3; tea. }
-    apply neuTerm; tea.
-    - assert ([Δ |-[ ta ] F[σ]]).
-      { now eapply escape, VF. }
-      eapply tm_ne_conv; [now eapply tm_ne_rel| |].
-      * replace F[_ >> _] with F[σ']⟨ρ⟩ by (unfold ρ; now bsimpl).
-        apply wft_wk; [eassumption|].
-        now eapply escape, VF.
-      * replace F[_ >> _] with (F[σ'])⟨↑⟩ by (unfold ρ; now bsimpl).
-        do 2 erewrite <- wk1_ren_on.
-        apply convty_wk; [tea|].
-        eapply escapeEq, VF; tea.
+      eapply WescapeEq;  unshelve eapply validTyExt; cycle 3; tea. }
+    apply WneuTerm; tea.
     - apply convneu_var; tea.
 Qed.
 
-Lemma liftSubstS' {Γ σ Δ lF F} {VΓ : [||-v Γ]} {wfΔ : [|- Δ]}
-  (VF : [Γ ||-v<lF> F | VΓ])
-  (Vσ : [Δ ||-v σ : Γ | VΓ | wfΔ ]) :
+Lemma liftSubstS' {wl Γ σ Δ lF F} {VΓ : [||-v Γ]< wl >} {wfΔ : [|- Δ]< wl >}
+  (VF : [Γ ||-v<lF> F | VΓ]< wl >)
+  (Vσ : [Δ ||-v σ : Γ | VΓ | wfΔ ]< wl >) :
   let VΓF := validSnoc VΓ VF in
-  let wfΔF := wfc_cons wfΔ (escape (validTy VF wfΔ Vσ)) in
-  [Δ ,, F[σ] ||-v up_term_term σ : Γ ,, F | VΓF | wfΔF ].
+  let wfΔF := wfc_cons wfΔ (Wescape (validTy VF wfΔ Vσ)) in
+  [Δ ,, F[σ] ||-v up_term_term σ : Γ ,, F | VΓF | wfΔF ]< wl >.
 Proof.
   eapply irrelevanceSubstExt.
   2: eapply liftSubstS.
   intros ?; now bsimpl.
 Qed.
 
-Lemma liftSubstSEq {Γ σ σ' Δ lF F} (VΓ : [||-v Γ]) (wfΔ : [|- Δ])
-  (VF : [Γ ||-v<lF> F | VΓ])
-  (Vσ : [Δ ||-v σ : Γ | VΓ | wfΔ ]) :
+Lemma liftSubstSEq {wl Γ σ σ' Δ lF F} (VΓ : [||-v Γ]< wl >) (wfΔ : [|- Δ]< wl >)
+  (VF : [Γ ||-v<lF> F | VΓ]< wl >)
+  (Vσ : [Δ ||-v σ : Γ | VΓ | wfΔ ]< wl >) :
   let VΓF := validSnoc VΓ VF in
   let ρ := @wk1 Δ F[σ] in
-  let wfΔF := wfc_cons wfΔ (escape (validTy VF wfΔ Vσ)) in
+  let wfΔF := wfc_cons wfΔ (Wescape (validTy VF wfΔ Vσ)) in
   let Vliftσ := liftSubstS VΓ wfΔ VF Vσ in
-  [Δ ||-v σ ≅ σ' : Γ | VΓ | wfΔ | Vσ] ->
-  [Δ ,, F[σ] ||-v (tRel 0 .: σ ⟨ ρ ⟩) ≅ (tRel 0 .: σ' ⟨ ρ ⟩) : Γ ,, F | VΓF | wfΔF | Vliftσ].
+  [Δ ||-v σ ≅ σ' : Γ | VΓ | wfΔ | Vσ]< wl > ->
+  [Δ ,, F[σ] ||-v (tRel 0 .: σ ⟨ ρ ⟩) ≅ (tRel 0 .: σ' ⟨ ρ ⟩) : Γ ,, F | VΓF | wfΔF | Vliftσ]< wl >.
 Proof.
   intros; unshelve econstructor.
   + now apply wk1SubstSEq.
-  + apply LREqTermRefl_; exact (validHead Vliftσ).
+  + apply WreflLRTmEq; exact (validHead Vliftσ).
 Qed.
 
-Lemma liftSubstSEq' {Γ σ σ' Δ lF F} {VΓ : [||-v Γ]} {wfΔ : [|- Δ]}
-  (VF : [Γ ||-v<lF> F | VΓ])
-  {Vσ : [Δ ||-v σ : Γ | VΓ | wfΔ ]} :
+Lemma liftSubstSEq' {wl Γ σ σ' Δ lF F} {VΓ : [||-v Γ]< wl >} {wfΔ : [|- Δ]< wl >}
+  (VF : [Γ ||-v<lF> F | VΓ]< wl >)
+  {Vσ : [Δ ||-v σ : Γ | VΓ | wfΔ ]< wl >} :
   let VΓF := validSnoc VΓ VF in
   let ρ := wk_up F (@wk_id Γ) in
-  let wfΔF := wfc_cons wfΔ (escape (validTy VF wfΔ Vσ)) in
+  let wfΔF := wfc_cons wfΔ (Wescape (validTy VF wfΔ Vσ)) in
   let Vliftσ := liftSubstS' VF Vσ in
-  [Δ ||-v σ ≅ σ' : Γ | VΓ | wfΔ | Vσ] ->
-  [Δ ,, F[σ] ||-v up_term_term σ ≅ up_term_term σ' : Γ ,, F | VΓF | wfΔF | Vliftσ].
+  [Δ ||-v σ ≅ σ' : Γ | VΓ | wfΔ | Vσ]< wl > ->
+  [Δ ,, F[σ] ||-v up_term_term σ ≅ up_term_term σ' : Γ ,, F | VΓF | wfΔF | Vliftσ]< wl >.
 Proof.
   intros.
   eapply irrelevanceSubstEq.
@@ -237,15 +234,15 @@ Proof.
   Unshelve. all: tea.
 Qed.
 
-Lemma liftSubstSrealign' {Γ σ σ' Δ lF F} {VΓ : [||-v Γ]} {wfΔ : [|- Δ]}
-  (VF : [Γ ||-v<lF> F | VΓ])
-  {Vσ : [Δ ||-v σ : Γ | VΓ | wfΔ ]} :
+Lemma liftSubstSrealign' {wl Γ σ σ' Δ lF F} {VΓ : [||-v Γ]< wl >} {wfΔ : [|- Δ]< wl >}
+  (VF : [Γ ||-v<lF> F | VΓ]< wl >)
+  {Vσ : [Δ ||-v σ : Γ | VΓ | wfΔ ]< wl >} :
   let VΓF := validSnoc VΓ VF in
   let ρ := wk_up F (@wk_id Γ) in
-  let wfΔF := wfc_cons wfΔ (escape (validTy VF wfΔ Vσ)) in
-  [Δ ||-v σ ≅ σ' : Γ | VΓ | wfΔ | Vσ] ->
-  [Δ ||-v σ' : Γ | VΓ | wfΔ ] ->
-  [Δ ,, F[σ] ||-v up_term_term σ' : Γ ,, F | VΓF | wfΔF].
+  let wfΔF := wfc_cons wfΔ (Wescape (validTy VF wfΔ Vσ)) in
+  [Δ ||-v σ ≅ σ' : Γ | VΓ | wfΔ | Vσ]< wl > ->
+  [Δ ||-v σ' : Γ | VΓ | wfΔ ]< wl > ->
+  [Δ ,, F[σ] ||-v up_term_term σ' : Γ ,, F | VΓF | wfΔF]< wl >.
 Proof.
   intros.
   eapply irrelevanceSubstExt.
@@ -253,80 +250,83 @@ Proof.
   intros ?; now bsimpl.
 Qed.
 
-Lemma wk1ValidTy {Γ lA A lF F} {VΓ : [||-v Γ]} (VF : [Γ ||-v<lF> F | VΓ]) :
-  [Γ ||-v<lA> A | VΓ] -> 
-  [Γ ,, F ||-v<lA> A ⟨ @wk1 Γ F ⟩ | validSnoc VΓ VF ].
+Lemma wk1ValidTy {wl Γ lA A lF F} {VΓ : [||-v Γ]< wl >} (VF : [Γ ||-v<lF> F | VΓ]< wl >) :
+  [Γ ||-v<lA> A | VΓ]< wl > -> 
+  [Γ ,, F ||-v<lA> A ⟨ @wk1 Γ F ⟩ | validSnoc VΓ VF ]< wl >.
 Proof.
   assert (forall σ, (A ⟨@wk1 Γ F⟩)[σ] = A[↑ >> σ]) as h by (intros; asimpl; now rewrite wk1_ren) ;
   intros [VA VAext]; unshelve econstructor.
   - abstract (intros * [tl _]; rewrite h; exact (VA _ _ wfΔ tl)).
   - intros * [tl _] [tleq _].
-    rewrite (h σ'); unshelve eapply LRTyEqSym.
+    rewrite (h σ'); unshelve eapply WLRTyEqSym.
     2: eapply VA; eassumption.
     rewrite (h σ).
     eapply VAext. 1: exact (validTail vσ).
     eapply symmetrySubstEq. eassumption.
 Qed.
 
-Lemma wk1ValidTyEq {Γ lA A B lF F} {VΓ : [||-v Γ]} (VF : [Γ ||-v<lF> F | VΓ]) 
-  {VA : [Γ ||-v<lA> A | VΓ]} :
-  [Γ ||-v<lA> A ≅ B | VΓ | VA] -> 
-  [Γ ,, F ||-v<lA> A ⟨ @wk1 Γ F ⟩ ≅ B ⟨ @wk1 Γ F ⟩ | validSnoc VΓ VF | wk1ValidTy VF VA].
+Lemma wk1ValidTyEq {wl Γ lA A B lF F} {VΓ : [||-v Γ]< wl >} (VF : [Γ ||-v<lF> F | VΓ]< wl >) 
+  {VA : [Γ ||-v<lA> A | VΓ]< wl >} :
+  [Γ ||-v<lA> A ≅ B | VΓ | VA]< wl > -> 
+  [Γ ,, F ||-v<lA> A ⟨ @wk1 Γ F ⟩ ≅ B ⟨ @wk1 Γ F ⟩ | validSnoc VΓ VF | wk1ValidTy VF VA]< wl >.
 Proof.
   assert (forall A σ, (A ⟨@wk1 Γ F⟩)[σ] = A[↑ >> σ]) as h by (intros; asimpl; now rewrite wk1_ren).
   intros []; constructor; intros.
-  rewrite h. irrelevance0.
-  1: symmetry; apply h.
-  unshelve intuition; tea; now eapply validTail.
+  Wirrelevance0 ; [symmetry ; now apply h | rewrite (h B) ].
+  unshelve eapply validTyEq ; [assumption | now eapply validTail ].
 Qed.
 
-Lemma wk1ValidTm {Γ lA t A lF F} {VΓ : [||-v Γ]}
-  (VF : [Γ ||-v<lF> F | VΓ])
-  (VA : [Γ ||-v<lA> A | VΓ])
-  (Vt : [Γ ||-v<lA> t : A | VΓ | VA]) (ρ := @wk1 Γ F):
-  [Γ,, F ||-v<lA> t⟨ρ⟩ : A⟨ρ⟩ | validSnoc VΓ VF | wk1ValidTy VF VA].
+Lemma wk1ValidTm {wl Γ lA t A lF F} {VΓ : [||-v Γ]< wl >}
+  (VF : [Γ ||-v<lF> F | VΓ]< wl >)
+  (VA : [Γ ||-v<lA> A | VΓ]< wl >)
+  (Vt : [Γ ||-v<lA> t : A | VΓ | VA]< wl >) (ρ := @wk1 Γ F):
+  [Γ,, F ||-v<lA> t⟨ρ⟩ : A⟨ρ⟩ | validSnoc VΓ VF | wk1ValidTy VF VA]< wl >.
 Proof.
   assert (forall A σ, (A ⟨@wk1 Γ F⟩)[σ] = A[↑ >> σ]) as h by (intros; asimpl; now rewrite wk1_ren).
   constructor; intros; repeat rewrite h.
-  - instValid (validTail Vσ); irrelevance.
-  - instValidExt (validTail Vσ') (eqTail Vσσ'); irrelevance.
+  - instValid (validTail Vσ) ; now Wirrelevance.
+  - instValidExt (validTail Vσ') (eqTail Vσσ') ; now Wirrelevance. 
 Qed.
 
-Lemma wk1ValidTmEq {Γ lA t u A lF F} {VΓ : [||-v Γ]}
-  (VF : [Γ ||-v<lF> F | VΓ])
-  (VA : [Γ ||-v<lA> A | VΓ])
-  (Vtu : [Γ ||-v<lA> t ≅ u : A | VΓ | VA]) (ρ := @wk1 Γ F):
-  [Γ,, F ||-v<lA> t⟨ρ⟩ ≅ u⟨ρ⟩ : A⟨ρ⟩ | validSnoc VΓ VF | wk1ValidTy VF VA].
+Lemma wk1ValidTmEq {wl Γ lA t u A lF F} {VΓ : [||-v Γ]< wl >}
+  (VF : [Γ ||-v<lF> F | VΓ]< wl >)
+  (VA : [Γ ||-v<lA> A | VΓ]< wl >)
+  (Vtu : [Γ ||-v<lA> t ≅ u : A | VΓ | VA]< wl >) (ρ := @wk1 Γ F):
+  [Γ,, F ||-v<lA> t⟨ρ⟩ ≅ u⟨ρ⟩ : A⟨ρ⟩ | validSnoc VΓ VF | wk1ValidTy VF VA]< wl >.
 Proof.
   assert (forall A σ, (A ⟨@wk1 Γ F⟩)[σ] = A[↑ >> σ]) as h by (intros; asimpl; now rewrite wk1_ren).
-  constructor; intros; repeat rewrite h.
-  instValid (validTail Vσ); irrelevance.
+  constructor; intros ; repeat rewrite h.
+  instValid (validTail Vσ); Wirrelevance.
+  now rewrite h.
 Qed.
 
 
-Lemma embValidTy@{u i j k l} {Γ l l' A}
-    {VΓ : [VR@{i j k l}| ||-v Γ]} (h : l << l')
-    (VA : typeValidity@{u i j k l} Γ VΓ l A (*[Γ ||-v<l> A |VΓ]*)) :
-    typeValidity@{u i j k l} Γ VΓ l' A (*[Γ ||-v<l'> A |VΓ]*).
+Lemma embValidTy@{u i j k l} {wl Γ l l' A}
+    {VΓ : [VR@{i j k l}| ||-v Γ]< wl >} (h : l << l')
+    (VA : typeValidity@{u i j k l} wl Γ VΓ l A (*[Γ ||-v<l> A |VΓ]< wl >*)) :
+    typeValidity@{u i j k l} wl Γ VΓ l' A (*[Γ ||-v<l'> A |VΓ]< wl >*).
 Proof.
   unshelve econstructor.
-  - intros ??? Vσ; destruct (validTy VA _  Vσ) as [pack]; exists pack.
-    eapply LR_embedding; tea.
-  - intros; now eapply validTyExt.
+  - intros ??? Vσ; destruct (validTy VA _  Vσ) as [d pack] ; exists d ; intros.
+    exists (pack wl' Ho) ; eapply LR_embedding ; tea.
+    now eapply pack.
+  - intros ; cbn. Wirrelevance0 ; [ reflexivity | unshelve eapply validTyExt].
+  3: eassumption.
+  all: tea.
 Defined.
 
-Lemma embValidTyOne @{u i j k l} {Γ l A}
-    {VΓ : [VR@{i j k l}| ||-v Γ]}
-    (VA : typeValidity@{u i j k l} Γ VΓ l A (*[Γ ||-v<l> A |VΓ]*)) :
-    typeValidity@{u i j k l} Γ VΓ one A (*[Γ ||-v<one> A |VΓ]*).
+Lemma embValidTyOne @{u i j k l} {wl Γ l A}
+    {VΓ : [VR@{i j k l}| ||-v Γ]< wl >}
+    (VA : typeValidity@{u i j k l} wl Γ VΓ l A (*[Γ ||-v<l> A |VΓ]*)) :
+    typeValidity@{u i j k l} wl Γ VΓ one A (*[Γ ||-v<one> A |VΓ]*).
 Proof.
   destruct l; tea; now eapply (embValidTy Oi).
 Defined.
 
-Lemma soundCtxId {Γ} (VΓ : [||-v Γ]) :
-  ∑ wfΓ : [|- Γ], [Γ ||-v tRel : Γ | VΓ | wfΓ].
+Lemma soundCtxId {wl Γ} (VΓ : [||-v Γ]< wl >) :
+  ∑ wfΓ : [|- Γ]< wl >, [Γ ||-v tRel : Γ | VΓ | wfΓ]< wl >.
 Proof.
-  enough (G : ∑ Δ (e : Δ = Γ) (wfΔ : [|-Δ]), [VΓ |Δ ||-v tRel : Γ | wfΔ]).
+  enough (G : ∑ Δ (e : Δ = Γ) (wfΔ : [|-Δ]< wl >), [VΓ |Δ ||-v tRel : Γ | wfΔ]< wl >).
   1: now destruct G as [? [-> ?]].
   pattern Γ, VΓ; apply validity_rect; clear Γ VΓ.
   - exists ε, eq_refl, wfc_nil; constructor.
@@ -335,19 +335,145 @@ Proof.
     1: asimpl; now rewrite e.
     unshelve eexists.
     + apply wfc_cons; tea.
-      eapply escape.
+      eapply Wescape.
       apply (validTy VA wfΔ Vid).
     + eapply irrelevanceSubstExt.
       2: eapply irrelevanceSubst; now unshelve eapply liftSubstS.
       intros []; [| bsimpl]; reflexivity.
 Qed.
 
-Definition soundCtx {Γ} (VΓ : [||-v Γ]) : [|-Γ] := (soundCtxId VΓ).π1.
+Definition soundCtx {wl Γ} (VΓ : [||-v Γ]< wl >) : [|-Γ]< wl > := (soundCtxId VΓ).π1.
 
-Definition idSubstS {Γ} (VΓ : [||-v Γ]) : [Γ ||-v tRel : Γ | VΓ | _] := (soundCtxId VΓ).π2.
+Definition idSubstS {wl Γ} (VΓ : [||-v Γ]< wl >) : [Γ ||-v tRel : Γ | VΓ | _]< wl > := (soundCtxId VΓ).π2.
 
-Lemma reflIdSubstS {Γ} (VΓ : [||-v Γ]) : [Γ ||-v tRel ≅ tRel : Γ | VΓ | _ | idSubstS VΓ].
+Lemma reflIdSubstS {wl Γ} (VΓ : [||-v Γ]< wl >) : [Γ ||-v tRel ≅ tRel : Γ | VΓ | _ | idSubstS VΓ]< wl >.
 Proof.  apply reflSubst. Qed.
+
+Lemma substS_wk {wl Γ Δ} (ρ : Δ ≤ Γ) :
+  forall (VΓ : [||-v Γ]< wl >)
+  (VΔ : [||-v Δ]< wl >) 
+  {Ξ σ} (wfΞ : [|- Ξ]< wl >), [VΔ | Ξ ||-v σ : _ | wfΞ]< wl > -> [VΓ | Ξ ||-v ρ >> σ : _ | wfΞ]< wl >.
+Proof.
+  destruct ρ as [? wwk]; induction wwk.
+  + intros; rewrite (invValidityEmpty VΓ); constructor.
+  + intros.
+    pose proof (invValiditySnoc VΔ) as [? [? [? eq]]].
+    rewrite eq in X; cbn in X; inversion X.
+    eapply irrelevanceSubstExt.
+    1: rewrite <- (scons_eta' σ); reflexivity.
+    cbn. asimpl.
+    now eapply IHwwk.
+  + intros.
+    pose proof (invValiditySnoc VΔ) as [? [? [? eq]]].
+    rewrite eq in X; cbn in X; inversion X.
+    eapply irrelevanceSubstExt.
+    1:{ rewrite <- (scons_eta' σ); cbn; unfold up_ren; rewrite scons_comp'; cbn. reflexivity. }
+    asimpl.
+    pose proof (invValiditySnoc VΓ) as [? [? [? eq']]].
+    rewrite eq'.
+    unshelve eapply consSubstS.
+    * now eapply IHwwk.
+    * Wirrelevance.
+Defined.
+
+Lemma substSEq_wk {wl Γ Δ} (ρ : Δ ≤ Γ) :
+  forall (VΓ : [||-v Γ]< wl >)
+  (VΔ : [||-v Δ]< wl >) 
+  Ξ σ σ' (wfΞ : [|- Ξ]< wl >)
+  (Vσ : [VΔ | Ξ ||-v σ : _ | wfΞ]< wl >),
+  [VΔ | Ξ ||-v σ' : _ | wfΞ]< wl > -> 
+  [VΔ | Ξ ||-v σ ≅ σ' : _ | wfΞ | Vσ]< wl > -> 
+  [VΓ | Ξ ||-v ρ >> σ ≅ ρ >> σ' : _ | wfΞ | substS_wk ρ VΓ VΔ wfΞ Vσ]< wl >.
+Proof.
+  destruct ρ as [? wwk]; induction wwk.
+  + intros; rewrite (invValidityEmpty VΓ); constructor.
+  + intros.
+    pose proof (invValiditySnoc VΔ) as [? [? [? eq]]].
+    revert Vσ X X0; rewrite eq; intros Vσ Vσ' Vσσ'.
+    cbn; asimpl; eapply irrelevanceSubstEq.
+    unshelve eapply IHwwk; tea.
+    1,2: now eapply validTail.
+    now eapply eqTail.
+    Unshelve. tea.
++ intros ??????.
+  set (ρ0 := {| well_wk := _ |}); unfold ρ0.
+  pose proof (invValiditySnoc VΔ) as [? [VΓ0 [? eq]]].
+  pose proof (invValiditySnoc VΓ) as [? [VΔ0 [? eqΓ]]].
+  rewrite eq; intros Vσ Vσ' Vσσ'.
+  assert (subst_eq : forall τ : nat -> term, τ var_zero .: (ρ >> ↑ >> τ) =1 (0 .: ρ >> S) >> τ).
+  1:{ intros τ;  asimpl; reflexivity. }
+  pose proof (v := substS_wk ρ0 VΓ _ wfΞ Vσ).
+  cbn; asimpl ; eapply irrelevanceSubstEq; unshelve eapply irrelevanceSubstEqExt.
+  2,5: apply subst_eq.
+  - eapply irrelevanceSubstExt.
+    1: symmetry; apply subst_eq.
+    exact v.
+  - eapply irrelevanceSubstEq.
+    eapply consSubstSEq'.
+    * exact (IHwwk VΔ0 VΓ0 Ξ (↑ >> σ) (↑ >> σ') wfΞ (validTail Vσ) (validTail Vσ') (eqTail Vσσ')).
+    * Wirrelevance0. 
+      2: now eapply eqHead. 
+      now asimpl.
+    Unshelve. 2: tea.
+    rewrite eqΓ in v.
+    Wirrelevance0 ; [reflexivity | ].
+    eapply (validHead v).
+Qed.
+
+Lemma wkValidTy {l wl Γ Δ A} (ρ : Δ ≤ Γ)
+  (VΓ : [||-v Γ]< wl >)
+  (VΔ : [||-v Δ]< wl >)
+  (VA : [Γ ||-v<l> A | VΓ]< wl >) :
+  [Δ ||-v<l> A⟨ρ⟩ | VΔ]< wl >.
+Proof.
+  assert (h : forall σ, A⟨ρ⟩[σ] = A[ ρ >> σ]) by (intros; now asimpl).
+  unshelve econstructor.
+  - intros; rewrite h.
+    eapply validTy; tea.
+    now eapply substS_wk.
+  - intros; Wirrelevance0; rewrite h; [reflexivity|].
+    eapply validTyExt.
+    1: now eapply substS_wk.
+    now eapply substSEq_wk.
+    Unshelve. 2,3: tea.
+Qed.
+
+Lemma wkValidTm {l wl Γ Δ A t} (ρ : Δ ≤ Γ)
+  (VΓ : [||-v Γ]< wl >)
+  (VΔ : [||-v Δ]< wl >)
+  (VA : [Γ ||-v<l> A | VΓ]< wl >)
+  (Vt : [Γ ||-v<l> t : A | VΓ | VA]< wl >) :
+  [Δ ||-v<l> t⟨ρ⟩ : A⟨ρ⟩ | VΔ | wkValidTy ρ VΓ VΔ VA]< wl >.
+Proof.
+  assert (hA : forall σ, A⟨ρ⟩[σ] = A[ρ >> σ]) by (intros; now asimpl).
+  assert (ht : forall σ, t⟨ρ⟩[σ] = t[ρ >> σ]) by (intros; now asimpl).
+  unshelve econstructor.
+  - intros; rewrite ht.
+    Wirrelevance0; [symmetry; apply hA|].
+    eapply validTm, Vt.
+  - intros; do 2 rewrite ht.
+    Wirrelevance0; [symmetry; apply hA|].
+    eapply validTmExt; [apply Vt|now eapply substS_wk|].
+    now eapply substSEq_wk.
+    Unshelve. all: tea.
+    now eapply substS_wk.
+Qed.
+
+Lemma wkValidTyEq {l wl Γ Δ A B} (ρ : Δ ≤ Γ)
+  (VΓ : [||-v Γ]< wl >)
+  (VΔ : [||-v Δ]< wl >)
+  (VA : [Γ ||-v<l> A | VΓ]< wl >)
+  (VAB : [Γ ||-v<l> A ≅ B | VΓ | VA]< wl >) :
+  [Δ ||-v<l> A⟨ρ⟩ ≅ B⟨ρ⟩ | VΔ | wkValidTy ρ VΓ VΔ VA]< wl >.
+Proof.
+  assert (h : forall A σ, A⟨ρ⟩[σ] = A[ ρ >> σ]) by (intros; now asimpl).
+  unshelve econstructor; intros; Wirrelevance0; rewrite h; [reflexivity|].
+  now eapply validTyEq.
+  Unshelve. 1: tea.
+    now eapply substS_wk.
+Qed.
+
+
 
 
 End Properties.
