theories/Validity.v
@@ -1,5 +1,5 @@
 From LogRel.AutoSubst Require Import core unscoped Ast Extra.
-From LogRel Require Import Utils BasicAst Notations Context NormalForms Weakening GenericTyping LogicalRelation.
+From LogRel Require Import Utils BasicAst Notations LContexts Context NormalForms Weakening GenericTyping LogicalRelation.
 
 Set Primitive Projections.
 Set Universe Polymorphism.
@@ -18,21 +18,21 @@ Ltac substitution := eauto with substitution.
   One should think of VRel as a functional relation taking one argument Γ and returning
   2 outputs validSubst and eqSubst *)
 
-  Definition VRel@{i j | i < j +} `{ta : tag} `{!WfContext ta} :=
-  forall
-    (Γ : context)
-    (validSubst : forall (Δ : context) (σ : nat -> term) (wfΔ : [|- Δ]), Type@{i})
-    (eqSubst : forall (Δ : context) (σ σ' : nat -> term) (wfΔ : [|- Δ ]), validSubst Δ σ wfΔ -> Type@{i})
+  Definition VRel@{i j | i < j +} `{ta : tag} `{!WfContext ta} {wl : wfLCon} :=
+    forall
+      (Γ : context)
+      (validSubst : forall (Δ : context) (σ : nat -> term) (wfΔ : [|- Δ]< wl >), Type@{i})
+      (eqSubst : forall (Δ : context) (σ σ' : nat -> term) (wfΔ : [|- Δ ]< wl >), validSubst Δ σ wfΔ -> Type@{i})
     , Type@{j}.
 
 (* A VPack contains the data corresponding to the codomain of VRel seen as a functional relation *)
 
 Module VPack.
 
-  Record VPack@{i} `{ta : tag} `{!WfContext ta} {Γ : context} :=
+  Record VPack@{i} `{ta : tag} `{!WfContext ta} {wl : wfLCon} {Γ : context} :=
   {
-    validSubst : forall (Δ : context) (σ : nat -> term) (wfΔ : [|- Δ]), Type@{i} ;
-    eqSubst : forall (Δ : context) (σ σ' : nat -> term) (wfΔ : [|- Δ ]), validSubst Δ σ wfΔ -> Type@{i} ;
+    validSubst : forall (Δ : context) (σ : nat -> term) (wfΔ : [|- Δ]< wl >), Type@{i} ;
+    eqSubst : forall (Δ : context) (σ σ' : nat -> term) (wfΔ : [|- Δ ]< wl >), validSubst Δ σ wfΔ -> Type@{i} ;
   }.
 
   Arguments VPack : clear implicits.
@@ -42,27 +42,27 @@ End VPack.
 
 Export VPack(VPack,Build_VPack).
 
-Notation "[ P | Δ ||-v σ : Γ | wfΔ ]" := (@VPack.validSubst _ _ Γ P Δ σ wfΔ) (at level 0, P, Δ, σ, Γ, wfΔ at level 50).
-Notation "[ P | Δ ||-v σ ≅ σ' : Γ | wfΔ | vσ ]" := (@VPack.eqSubst _ _ Γ P Δ σ σ' wfΔ vσ) (at level 0, P, Δ, σ, σ', Γ, wfΔ, vσ at level 50).
+Notation "[ P | Δ ||-v σ : Γ | wfΔ ]< wl >" := (@VPack.validSubst _ _ wl Γ P Δ σ wfΔ) (at level 0, P, Δ, σ, wl, Γ, wfΔ at level 50).
+Notation "[ P | Δ ||-v σ ≅ σ' : Γ | wfΔ | vσ ]< wl >" := (@VPack.eqSubst _ _ wl Γ P Δ σ σ' wfΔ vσ) (at level 0, P, Δ, σ, σ', wl, Γ, wfΔ, vσ at level 50).
 
 (* An VPack it adequate wrt. a VRel when its three unpacked components are *)
-#[universes(polymorphic)] Definition VPackAdequate@{i j} `{ta : tag} `{!WfContext ta} {Γ : context}
-  (R : VRel@{i j}) (P : VPack@{i} Γ) : Type@{j} :=
+#[universes(polymorphic)] Definition VPackAdequate@{i j} `{ta : tag} `{!WfContext ta} {wl : wfLCon} {Γ : context}
+  (R : VRel@{i j}) (P : VPack@{i} wl Γ) : Type@{j} :=
   R Γ P.(VPack.validSubst) P.(VPack.eqSubst).
 
 Arguments VPackAdequate _ _ /.
 
 Module VAd.
 
-  Record > VAdequate `{ta : tag} `{!WfContext ta} {Γ : context} {R : VRel} :=
+  Record > VAdequate `{ta : tag} `{!WfContext ta} {wl : wfLCon} {Γ : context} {R : VRel} :=
   {
-    pack :> VPack Γ ;
+    pack :> VPack wl Γ ;
     adequate :> VPackAdequate R pack
   }.
 
   Arguments VAdequate : clear implicits.
   Arguments VAdequate {_ _}.
-  Arguments Build_VAdequate {_ _ _ _}.
+  Arguments Build_VAdequate {_ _ _ _ _}.
 
 End VAd.
 
@@ -72,199 +72,202 @@ Export VAd(VAdequate,Build_VAdequate).
 Coercion VAd.pack : VAdequate >-> VPack.
 Coercion VAd.adequate : VAdequate >-> VPackAdequate.
 
-Notation "[ R | ||-v Γ ]"                            := (VAdequate Γ R) (at level 0, R, Γ at level 50).
-Notation "[ R | Δ ||-v σ : Γ | RΓ | wfΔ ]"           := (RΓ.(@VAd.pack _ _ Γ R).(VPack.validSubst) Δ σ wfΔ) (at level 0, R, Δ, σ, Γ, RΓ, wfΔ at level 50).
-Notation "[ R | Δ ||-v σ ≅ σ' : Γ | RΓ | wfΔ | vσ ]" := (RΓ.(@VAd.pack _ _ Γ R).(VPack.eqSubst) Δ σ σ' wfΔ vσ) (at level 0, R, Δ, σ, σ', Γ, RΓ, wfΔ, vσ at level 50).
+Notation "[ R | ||-v Γ ]< wl >"                            := (VAdequate wl Γ R) (at level 0, R, wl, Γ at level 50).
+Notation "[ R | Δ ||-v σ : Γ | RΓ | wfΔ ]< wl >"           := (RΓ.(@VAd.pack _ _ wl Γ R).(VPack.validSubst) Δ σ wfΔ) (at level 0, R, Δ, σ, wl, Γ, RΓ, wfΔ at level 50).
+Notation "[ R | Δ ||-v σ ≅ σ' : Γ | RΓ | wfΔ | vσ ]< wl >" := (RΓ.(@VAd.pack _ _ wl Γ R).(VPack.eqSubst) Δ σ σ' wfΔ vσ) (at level 0, R, Δ, σ, σ', wl, Γ, RΓ, wfΔ, vσ at level 50).
 
 Record typeValidity@{u i j k l} `{ta : tag} `{!WfContext ta}
   `{!WfType ta} `{!Typing ta} `{!ConvType ta}
-  `{!ConvTerm ta} `{!ConvNeuConv ta} `{!RedType ta} `{!TypeNf ta} `{!TypeNe ta} `{!RedTerm ta} `{!TermNf ta} `{!TermNe ta}
-  {Γ : context} {VΓ : VPack@{u} Γ}
+  `{!ConvTerm ta} `{!ConvNeuConv ta} `{!RedType ta} `{!RedTerm ta}
+  {wl : wfLCon} {Γ : context} {VΓ : VPack@{u} wl Γ}
   {l : TypeLevel} {A : term} :=
   {
     validTy : forall {Δ : context} {σ : nat -> term}
-      (wfΔ : [|- Δ ])
-      (vσ : [ VΓ | Δ ||-v σ : Γ | wfΔ ])
-      , [LogRel@{i j k l} l | Δ ||- A [ σ ] ] ;
+      (wfΔ : [|- Δ ]< wl >)
+      (vσ : [ VΓ | Δ ||-v σ : Γ | wfΔ ]< wl >)
+      , WLogRel@{i j k l} l wl Δ (A [ σ ]);
     validTyExt : forall {Δ : context} {σ σ' : nat -> term}
-      (wfΔ : [|- Δ ])
-      (vσ  : [ VΓ | Δ ||-v σ  : Γ | wfΔ ])
-      (vσ' : [ VΓ | Δ ||-v σ' : Γ | wfΔ ])
-      (vσσ' : [ VΓ | Δ ||-v σ ≅ σ' : Γ | wfΔ | vσ ])
-      , [LogRel@{i j k l} l | Δ ||- A [ σ ] ≅ A [ σ' ] | validTy wfΔ vσ ]
+      (wfΔ : [|- Δ ]< wl >)
+      (vσ  : [ VΓ | Δ ||-v σ  : Γ | wfΔ ]< wl >)
+      (vσ' : [ VΓ | Δ ||-v σ' : Γ | wfΔ ]< wl >)
+      (vσσ' : [ VΓ | Δ ||-v σ ≅ σ' : Γ | wfΔ | vσ ]< wl >)
+      , WLogRelEq@{i j k l} l wl Δ (A [ σ ]) (A [ σ' ]) (validTy wfΔ vσ)
   }.
 
 Arguments typeValidity : clear implicits.
-Arguments typeValidity {_ _ _ _ _ _ _ _ _ _ _ _ _}.
+Arguments typeValidity {_ _ _ _ _ _ _ _ _}.
 
-Notation "[ P | Γ ||-v< l > A ]" := (typeValidity Γ P l A) (at level 0, P, Γ, l, A at level 50).
+Notation "[ P | Γ ||-v< l > A ]< wl >" := (typeValidity wl Γ P l A) (at level 0, P, wl, Γ, l, A at level 50).
 
-Definition emptyValidSubst `{ta : tag} `{!WfContext ta} : forall (Δ : context) (σ : nat -> term) (wfΔ : [|- Δ]), Type := fun _ _ _ => unit.
-Definition emptyEqSubst@{u} `{ta : tag} `{!WfContext ta} : forall (Δ : context) (σ σ' : nat -> term) (wfΔ : [|- Δ]), emptyValidSubst@{u} Δ σ wfΔ -> Type@{u} := fun _ _ _ _ _ => unit.
-Definition emptyVPack `{ta : tag} `{!WfContext ta} : VPack ε :=
-  Build_VPack _ emptyValidSubst emptyEqSubst.
+Definition emptyValidSubst `{ta : tag} `{!WfContext ta} {wl : wfLCon} : forall (Δ : context) (σ : nat -> term) (wfΔ : [|- Δ]< wl >), Type := fun _ _ _ => unit.
+Definition emptyEqSubst@{u} `{ta : tag} `{!WfContext ta} {wl : wfLCon} : forall (Δ : context) (σ σ' : nat -> term) (wfΔ : [|- Δ]< wl >), emptyValidSubst@{u} Δ σ wfΔ -> Type@{u} := fun _ _ _ _ _ => unit.
+Definition emptyVPack `{ta : tag} `{!WfContext ta} {wl : wfLCon} : VPack wl ε :=
+  Build_VPack _ _ emptyValidSubst emptyEqSubst.
 
 Section snocValid.
   Universe u i j k l.
   Context `{ta : tag} `{!WfContext ta}
   `{!WfType ta} `{!Typing ta} `{!ConvType ta}
-  `{!ConvTerm ta} `{!ConvNeuConv ta} `{!RedType ta} `{!TypeNf ta} `{!TypeNe ta} `{!RedTerm ta}  `{!TermNf ta} `{!TermNe ta}
-  {Γ : context} {VΓ : VPack@{u} Γ} {A : term} {l : TypeLevel}
-  {vA : typeValidity@{u i j k l} Γ VΓ l A (* [ VΓ | Γ ||-v< l > A ] *)}.
+  `{!ConvTerm ta} `{!ConvNeuConv ta} `{!RedType ta} `{!RedTerm ta}
+  {wl : wfLCon} {Γ : context} {VΓ : VPack@{u} wl Γ} {A : term} {l : TypeLevel}
+  {vA : typeValidity@{u i j k l} wl Γ VΓ l A (* [ VΓ | Γ ||-v< l > A ]< wl > *)}.
 
-  Record snocValidSubst {Δ : context} {σ : nat -> term} {wfΔ : [|- Δ]} : Type :=
+  Record snocValidSubst {Δ : context} {σ : nat -> term} {wfΔ : [|- Δ]< wl >} : Type :=
     {
-      validTail : [ VΓ | Δ ||-v ↑ >> σ : Γ | wfΔ ] ;
-      validHead : [ Δ ||-< l > σ var_zero : A[↑ >> σ] | validTy vA wfΔ validTail ]
+      validTail : [ VΓ | Δ ||-v ↑ >> σ : Γ | wfΔ ]< wl > ;
+      validHead : W[ Δ ||-< l > σ var_zero : A[↑ >> σ] | validTy vA wfΔ validTail ]< wl >
     }.
 
   Arguments snocValidSubst : clear implicits.
 
-  Record snocEqSubst {Δ : context} {σ σ' : nat -> term} {wfΔ : [|- Δ]} {vσ : snocValidSubst Δ σ wfΔ} : Type :=
+  Record snocEqSubst {Δ : context} {σ σ' : nat -> term} {wfΔ : [|- Δ]< wl >} {vσ : snocValidSubst Δ σ wfΔ} : Type :=
     {
-      eqTail : [ VΓ | Δ ||-v ↑ >> σ ≅ ↑ >> σ' : Γ | wfΔ | validTail vσ ] ;
-      eqHead : [ Δ ||-< l > σ var_zero ≅ σ' var_zero : A[↑ >> σ] | validTy vA wfΔ (validTail vσ) ]
+      eqTail : [ VΓ | Δ ||-v ↑ >> σ ≅ ↑ >> σ' : Γ | wfΔ | validTail vσ ]< wl > ;
+      eqHead : W[ Δ ||-< l > σ var_zero ≅ σ' var_zero : A[↑ >> σ] | validTy vA wfΔ (validTail vσ) ]< wl >
     }.
 
-  Definition snocVPack := Build_VPack@{u (* max(u,k) *)} (Γ ,, A) snocValidSubst (@snocEqSubst).
+  Definition snocVPack := Build_VPack@{u (* max(u,k) *)} wl (Γ ,, A) snocValidSubst (@snocEqSubst).
 End snocValid.
 
+
 Arguments snocValidSubst : clear implicits.
-Arguments snocValidSubst {_ _ _ _ _ _ _ _ _ _ _ _ _}.
+Arguments snocValidSubst {_ _ _ _ _ _ _ _ _}.
 
 Arguments snocEqSubst : clear implicits.
-Arguments snocEqSubst {_ _ _ _ _ _ _ _ _ _ _ _ _}.
+Arguments snocEqSubst {_ _ _ _ _ _ _ _ _}.
 
 Arguments snocVPack : clear implicits.
-Arguments snocVPack {_ _ _ _ _ _ _ _ _ _ _ _ _}.
+Arguments snocVPack {_ _ _ _ _ _ _ _ _}.
 
 Unset Elimination Schemes.
 
 Inductive VR@{i j k l} `{ta : tag}
   `{WfContext ta} `{WfType ta} `{Typing ta}
   `{ConvType ta} `{ConvTerm ta} `{ConvNeuConv ta}
-  `{RedType ta} `{!TypeNf ta} `{!TypeNe ta} `{RedTerm ta} `{!TermNf ta} `{!TermNe ta} : VRel@{k l} :=
+  `{RedType ta} `{RedTerm ta} {wl : wfLCon} : VRel@{k l} :=
   | VREmpty : VR ε emptyValidSubst@{k} emptyEqSubst@{k}
   | VRSnoc : forall {Γ A l}
-    (VΓ : VPack@{k} Γ)
+    (VΓ : VPack@{k} wl Γ)
     (VΓad : VPackAdequate@{k l} VR VΓ)
-    (VA : typeValidity@{k i j k l} Γ VΓ l A (*[ VΓ | Γ ||-v< l > A ]*)),
-    VR (Γ ,, A) (snocValidSubst Γ VΓ A l VA) (snocEqSubst Γ VΓ A l VA).
+    (VA : typeValidity@{k i j k l} wl Γ VΓ l A (*[ VΓ | Γ ||-v< l > A ]*)),
+    VR (Γ ,, A) (snocValidSubst wl Γ VΓ A l VA) (snocEqSubst wl Γ VΓ A l VA).
 
 
 Set Elimination Schemes.
 
-Notation "[||-v Γ ]"                             := [ VR | ||-v Γ ] (at level 0, Γ at level 50).
-Notation "[ Δ ||-v σ : Γ | VΓ | wfΔ ]"           := [ VR | Δ ||-v σ : Γ | VΓ | wfΔ ]  (at level 0, Δ, σ, Γ, VΓ, wfΔ at level 50).
-Notation "[ Δ ||-v σ ≅ σ' : Γ | VΓ | wfΔ | vσ ]" := [ VR | Δ ||-v σ ≅ σ' : Γ | VΓ | wfΔ | vσ ] (at level 0, Δ, σ, σ', Γ, VΓ, wfΔ, vσ at level 50).
-Notation "[ Γ ||-v< l > A | VΓ ]"                := [ VΓ | Γ ||-v< l > A ] (at level 0, Γ, l , A, VΓ at level 50).
+Notation "[||-v Γ ]< wl >"                             := [ VR | ||-v Γ ]< wl > (at level 0, wl, Γ at level 50).
+Notation "[ Δ ||-v σ : Γ | VΓ | wfΔ ]< wl >"           := [ VR | Δ ||-v σ : Γ | VΓ | wfΔ ]< wl >  (at level 0, Δ, σ, wl, Γ, VΓ, wfΔ at level 50).
+Notation "[ Δ ||-v σ ≅ σ' : Γ | VΓ | wfΔ | vσ ]< wl >" := [ VR | Δ ||-v σ ≅ σ' : Γ | VΓ | wfΔ | vσ ]< wl > (at level 0, Δ, σ, σ', wl, Γ, VΓ, wfΔ, vσ at level 50).
+Notation "[ Γ ||-v< l > A | VΓ ]< wl >"                := [ VΓ | Γ ||-v< l > A ]< wl > (at level 0, wl, Γ, l , A, VΓ at level 50).
 
 
 Section MoreDefs.
   Context `{ta : tag} `{WfContext ta} `{WfType ta} `{Typing ta}
-  `{ConvType ta} `{ConvTerm ta} `{ConvNeuConv ta} `{RedType ta} `{!TypeNf ta} `{!TypeNe ta} `{RedTerm ta} `{!TermNf ta} `{!TermNe ta}.
+  `{ConvType ta} `{ConvTerm ta} `{ConvNeuConv ta} `{RedType ta} `{RedTerm ta}.
 
-  Definition validEmpty@{i j k l} : [VR@{i j k l}| ||-v ε ] := Build_VAdequate emptyVPack VREmpty.
+  Definition validEmpty@{i j k l} {wl } : [VR@{i j k l}| ||-v ε ]< wl > := Build_VAdequate emptyVPack VREmpty.
 
-  Definition validSnoc@{i j k l} {Γ} {A l}
-    (VΓ : [VR@{i j k l}| ||-v Γ]) (VA : [Γ ||-v< l > A | VΓ])
-    : [||-v Γ ,, A ] :=
-    Build_VAdequate (snocVPack Γ VΓ A l VA) (VRSnoc VΓ VΓ VA).
+  Definition validSnoc@{i j k l} {wl Γ} {A l}
+    (VΓ : [VR@{i j k l}| ||-v Γ]< wl >) (VA : [Γ ||-v< l > A | VΓ]< wl >)
+    : [||-v Γ ,, A ]< wl > :=
+    Build_VAdequate (snocVPack wl Γ VΓ A l VA) (VRSnoc VΓ VΓ VA).
 
-  Record termValidity@{i j k l} {Γ l} {t A : term}
-    {VΓ : [VR@{i j k l}| ||-v Γ]}
-    {VA : typeValidity@{k i j k l} Γ VΓ l A (*[Γ ||-v<l> A |VΓ]*)} : Type :=
+  Record termValidity@{i j k l} {wl Γ l} {t A : term}
+    {VΓ : [VR@{i j k l} (wl := wl) | ||-v Γ]< wl >}
+    {VA : typeValidity@{k i j k l} wl Γ VΓ l A (*[Γ ||-v<l> A |VΓ]< wl >*)} : Type :=
     {
       validTm : forall {Δ σ}
-        (wfΔ : [|- Δ]) (Vσ : [Δ ||-v σ : Γ | VΓ | wfΔ]),
-        [Δ ||-<l> t[σ] : A[σ] | validTy VA wfΔ Vσ ] ;
+        (wfΔ : [|- Δ]< wl >) (Vσ : [Δ ||-v σ : Γ | VΓ | wfΔ]< wl >),
+        W[Δ ||-<l> t[σ] : A[σ] | validTy VA wfΔ Vσ ]< wl > ;
       validTmExt : forall {Δ : context} {σ σ' : nat -> term}
-        (wfΔ : [|- Δ ])
-        (Vσ  : [Δ ||-v σ  : Γ | VΓ | wfΔ ])
-        (Vσ' : [ Δ ||-v σ' : Γ | VΓ | wfΔ ])
-        (Vσσ' : [ Δ ||-v σ ≅ σ' : Γ | VΓ | wfΔ | Vσ ]),
-        [Δ ||-<l> t[σ] ≅ t[σ'] : A[σ] | validTy VA wfΔ Vσ ]
+        (wfΔ : [|- Δ ]< wl >)
+        (Vσ  : [Δ ||-v σ  : Γ | VΓ | wfΔ ]< wl >)
+        (Vσ' : [ Δ ||-v σ' : Γ | VΓ | wfΔ ]< wl >)
+        (Vσσ' : [ Δ ||-v σ ≅ σ' : Γ | VΓ | wfΔ | Vσ ]< wl >),
+        W[Δ ||-<l> t[σ] ≅ t[σ'] : A[σ] | validTy VA wfΔ Vσ ]< wl >
     }.
 
-  Record typeEqValidity@{i j k l} {Γ l} {A B : term}
-    {VΓ : [VR@{i j k l}| ||-v Γ]}
-    {VA : typeValidity@{k i j k l} Γ VΓ l A (*[Γ ||-v<l> A |VΓ]*)} : Type :=
+  Record typeEqValidity@{i j k l} {wl Γ l} {A B : term}
+    {VΓ : [VR@{i j k l}| ||-v Γ]< wl >}
+    {VA : typeValidity@{k i j k l} wl Γ VΓ l A (*[Γ ||-v<l> A |VΓ]< wl >*)} : Type :=
     {
       validTyEq : forall {Δ σ}
-        (wfΔ : [|- Δ]) (Vσ : [Δ ||-v σ : Γ | VΓ | wfΔ]),
-        [Δ ||-<l> A[σ] ≅ B[σ] | validTy VA wfΔ Vσ]
+        (wfΔ : [|- Δ]< wl >) (Vσ : [Δ ||-v σ : Γ | VΓ | wfΔ]< wl >),
+        W[Δ ||-<l> A[σ] ≅ B[σ] | validTy VA wfΔ Vσ]< wl >
     }.
 
-  Record termEqValidity@{i j k l} {Γ l} {t u A : term}
-    {VΓ : [VR@{i j k l}| ||-v Γ]}
-    {VA : typeValidity@{k i j k l} Γ VΓ l A (*[Γ ||-v<l> A |VΓ]*)} : Type :=
+  Record termEqValidity@{i j k l} {wl Γ l} {t u A : term}
+    {VΓ : [VR@{i j k l}| ||-v Γ]< wl >}
+    {VA : typeValidity@{k i j k l} wl Γ VΓ l A (*[Γ ||-v<l> A |VΓ]< wl >*)} : Type :=
     {
       validTmEq : forall {Δ σ}
-        (wfΔ : [|- Δ]) (Vσ : [Δ ||-v σ : Γ | VΓ | wfΔ]),
-        [Δ ||-<l> t[σ] ≅ u[σ] : A[σ] | validTy VA wfΔ Vσ]
+        (wfΔ : [|- Δ]< wl >) (Vσ : [Δ ||-v σ : Γ | VΓ | wfΔ]< wl >),
+        W[Δ ||-<l> t[σ] ≅ u[σ] : A[σ] | validTy VA wfΔ Vσ]< wl >
     }.
 
-  Record tmEqValidity {Γ l} {t u A : term} {VΓ : [||-v Γ]} : Type :=
+  Record tmEqValidity {wl Γ l} {t u A : term} {VΓ : [||-v Γ]< wl >} : Type :=
     {
-      Vty  : [Γ ||-v< l > A | VΓ] ;
-      Vlhs : @termValidity Γ l t A VΓ Vty ;
-      Vrhs : @termValidity Γ l u A VΓ Vty ;
-      Veq  : @termEqValidity Γ l t u A VΓ Vty
+      Vty  : [Γ ||-v< l > A | VΓ]< wl > ;
+      Vlhs : @termValidity wl Γ l t A VΓ Vty ;
+      Vrhs : @termValidity wl Γ l u A VΓ Vty ;
+      Veq  : @termEqValidity wl Γ l t u A VΓ Vty
     }.
 
-  Record redValidity {Γ} {t u A : term} {VΓ : [||-v Γ]} : Type :=
+  Record redValidity {wl Γ} {t u A : term} {VΓ : [||-v Γ]< wl >} : Type :=
     {
       validRed : forall {Δ σ}
-        (wfΔ : [|- Δ]) (Vσ : [Δ ||-v σ : Γ | VΓ | wfΔ]),
-        [Δ |- t[σ] :⇒*: u[σ] : A[σ]]
+        (wfΔ : [|- Δ]< wl >) (Vσ : [Δ ||-v σ : Γ | VΓ | wfΔ]< wl >),
+        [Δ |- t[σ] :⤳*: u[σ] : A[σ]]< wl >
     }.
 End MoreDefs.
 
 Arguments termValidity : clear implicits.
-Arguments termValidity {_ _ _ _ _ _ _ _ _ _ _ _ _}.
-Arguments Build_termValidity {_ _ _ _ _ _ _ _ _ _ _ _ _}.
+Arguments termValidity {_ _ _ _ _ _ _ _ _}.
+Arguments Build_termValidity {_ _ _ _ _ _ _ _ _}.
 
 Arguments typeEqValidity : clear implicits.
-Arguments typeEqValidity {_ _ _ _ _ _ _ _ _ _ _ _ _}.
-Arguments Build_typeEqValidity {_ _ _ _ _ _ _ _ _ _ _ _ _}.
+Arguments typeEqValidity {_ _ _ _ _ _ _ _ _}.
+Arguments Build_typeEqValidity {_ _ _ _ _ _ _ _ _}.
 
 Arguments termEqValidity : clear implicits.
-Arguments termEqValidity {_ _ _ _ _ _ _ _ _ _ _ _ _}.
-Arguments Build_termEqValidity {_ _ _ _ _ _ _ _ _ _ _ _ _}.
+Arguments termEqValidity {_ _ _ _ _ _ _ _ _}.
+Arguments Build_termEqValidity {_ _ _ _ _ _ _ _ _}.
 
 Arguments tmEqValidity : clear implicits.
-Arguments tmEqValidity {_ _ _ _ _ _ _ _ _ _ _ _ _}.
-Arguments Build_tmEqValidity {_ _ _ _ _ _ _ _ _ _ _ _ _}.
+Arguments tmEqValidity {_ _ _ _ _ _ _ _ _}.
+Arguments Build_tmEqValidity {_ _ _ _ _ _ _ _ _}.
 
 Arguments redValidity : clear implicits.
-Arguments redValidity {_ _ _ _ _ _ _ _ _ _ _ _ _}.
-Arguments Build_redValidity {_ _ _ _ _ _ _ _ _ _ _ _ _}.
+Arguments redValidity {_ _ _ _ _ _ _ _ _}.
+Arguments Build_redValidity {_ _ _ _ _ _ _ _ _}.
 
-Notation "[ Γ ||-v< l > t : A | VΓ | VA ]"     := (termValidity Γ l t A VΓ VA) (at level 0, Γ, l, t, A, VΓ, VA at level 50).
-Notation "[ Γ ||-v< l > A ≅ B | VΓ | VA ]"     := (typeEqValidity Γ l A B VΓ VA) (at level 0, Γ, l, A, B, VΓ, VA at level 50).
-Notation "[ Γ ||-v< l > t ≅ u : A | VΓ | VA ]" := (termEqValidity Γ l t u A VΓ VA) (at level 0, Γ, l, t, u, A, VΓ, VA at level 50).
-Notation "[ Γ ||-v< l > t ≅ u : A | VΓ ]"      := (tmEqValidity Γ l t u A VΓ) (at level 0, Γ, l, t, u, A, VΓ at level 50).
-Notation "[ Γ ||-v t :⇒*: u : A | VΓ ]"      := (redValidity Γ t u A VΓ) (at level 0, Γ, t, u, A, VΓ at level 50).
+Notation "[ Γ ||-v< l > t : A | VΓ | VA ]< wl >"     := (termValidity wl Γ l t A VΓ VA) (at level 0, wl, Γ, l, t, A, VΓ, VA at level 50).
+Notation "[ Γ ||-v< l > A ≅ B | VΓ | VA ]< wl >"     := (typeEqValidity wl Γ l A B VΓ VA) (at level 0, wl, Γ, l, A, B, VΓ, VA at level 50).
+Notation "[ Γ ||-v< l > t ≅ u : A | VΓ | VA ]< wl >" := (termEqValidity wl Γ l t u A VΓ VA) (at level 0, wl, Γ, l, t, u, A, VΓ, VA at level 50).
+Notation "[ Γ ||-v< l > t ≅ u : A | VΓ ]< wl >"      := (tmEqValidity wl Γ l t u A VΓ) (at level 0, wl, Γ, l, t, u, A, VΓ at level 50).
+Notation "[ Γ ||-v t :⤳*: u : A | VΓ ]< wl >"      := (redValidity wl Γ t u A VΓ) (at level 0, wl, Γ, t, u, A, VΓ at level 50).
 
 Section Inductions.
   Context `{ta : tag} `{WfContext ta} `{WfType ta} `{Typing ta}
-  `{ConvType ta} `{ConvTerm ta} `{ConvNeuConv ta} `{RedType ta} `{!TypeNf ta} `{!TypeNe ta} `{RedTerm ta} `{!TermNf ta} `{!TermNe ta}.
-
-  Theorem VR_rect
+    `{ConvType ta} `{ConvTerm ta} `{ConvNeuConv ta} `{RedType ta} `{RedTerm ta}.
+  
+  Theorem VR_rect {wl}
     (P : forall {Γ vSubst vSubstExt}, VR Γ vSubst vSubstExt -> Type)
     (hε : P VREmpty)
     (hsnoc : forall {Γ A l VΓ VΓad VA},
-      P VΓad -> P (VRSnoc (Γ := Γ) (A := A) (l := l) VΓ VΓad VA)) :
+      P VΓad -> P (VRSnoc (wl := wl) (Γ := Γ) (A := A) (l := l) VΓ VΓad VA)) :
     forall {Γ vSubst vSubstExt} (VΓ : VR Γ vSubst vSubstExt), P VΓ.
   Proof.
-    fix ih 4; destruct VΓ; [exact hε | apply hsnoc; apply ih].
+    fix ih 4.
+    destruct VΓ; [exact hε | apply hsnoc].
+    now unshelve eapply ih.
   Defined.
 
-  Theorem validity_rect
-    (P : forall {Γ : context}, [||-v Γ] -> Type)
+  Theorem validity_rect {wl}
+    (P : forall {Γ : context}, [||-v Γ]< wl > -> Type)
     (hε : P validEmpty)
-    (hsnoc : forall {Γ A l} (VΓ : [||-v Γ]) (VA : [Γ ||-v< l > A | VΓ]), P VΓ -> P (validSnoc VΓ VA)) :
-    forall {Γ : context} (VΓ : [||-v Γ]), P VΓ.
+    (hsnoc : forall {Γ A l} (VΓ : [||-v Γ]< wl >) (VA : [Γ ||-v< l > A | VΓ]< wl >), P VΓ -> P (validSnoc VΓ VA)) :
+    forall {Γ : context} (VΓ : [||-v Γ]< wl >), P VΓ.
   Proof.
     intros Γ [[s eq] VΓad]; revert Γ s eq VΓad.
     apply VR_rect.
@@ -272,11 +275,11 @@ Section Inductions.
     - intros *; apply hsnoc.
   Defined.
 
-  Lemma invValidity {Γ} (VΓ : [||-v Γ]) :
-    match Γ as Γ return [||-v Γ] -> Type with
+  Lemma invValidity {wl Γ} (VΓ : [||-v Γ]< wl >) :
+    match Γ as Γ return [||-v Γ]< wl > -> Type with
     | nil => fun VΓ₀ => VΓ₀ = validEmpty
     | (A :: Γ)%list => fun VΓ₀ =>
-      ∑ l (VΓ : [||-v Γ]) (VA : [Γ ||-v< l > A | VΓ]), VΓ₀ = validSnoc VΓ VA
+      ∑ l (VΓ : [||-v Γ]< wl >) (VA : [Γ ||-v< l > A | VΓ]< wl >), VΓ₀ = validSnoc VΓ VA
     end VΓ.
   Proof.
     pattern Γ, VΓ. apply validity_rect.
@@ -284,11 +287,11 @@ Section Inductions.
     - intros; do 3 eexists; reflexivity.
   Qed.
 
-  Lemma invValidityEmpty (VΓ : [||-v ε]) : VΓ = validEmpty.
+  Lemma invValidityEmpty {wl} (VΓ : [||-v ε]< wl >) : VΓ = validEmpty.
   Proof. apply (invValidity VΓ). Qed.
 
-  Lemma invValiditySnoc {Γ A} (VΓ₀ : [||-v Γ ,, A ]) :
-      ∑ l (VΓ : [||-v Γ]) (VA : [Γ ||-v< l > A | VΓ]), VΓ₀ = validSnoc VΓ VA.
+  Lemma invValiditySnoc {wl Γ A} (VΓ₀ : [||-v Γ ,, A ]< wl >) :
+      ∑ l (VΓ : [||-v Γ]< wl >) (VA : [Γ ||-v< l > A | VΓ]< wl >), VΓ₀ = validSnoc VΓ VA.
   Proof. apply (invValidity VΓ₀). Qed.
 
 End Inductions.
@@ -297,26 +300,25 @@ End Inductions.
   valid substitions *)
 
 Definition wfCtxOfsubstS `{GenericTypingProperties}
-  `{TypeNf ta} `{TypeNe ta} `{TermNf ta} `{TermNe ta}
-  {Γ Δ σ} {VΓ : [||-v Γ]} {wfΔ : [|- Δ]} :
-  [Δ ||-v σ : Γ | VΓ | wfΔ] -> [|- Δ] := fun _ => wfΔ.
+  {wl Γ Δ σ} {VΓ : [||-v Γ]< wl >} {wfΔ : [|- Δ]< wl >} :
+  [Δ ||-v σ : Γ | VΓ | wfΔ]< wl > -> [|- Δ]< wl > := fun _ => wfΔ.
 
 Ltac instValid vσ :=
   let wfΔ := (eval unfold wfCtxOfsubstS in (wfCtxOfsubstS vσ)) in
   repeat lazymatch goal with
-  | [H : typeValidity _ _ _ _ |- _] =>
+  | [H : typeValidity _ _ _ _ _ |- _] =>
     let X := fresh "R" H in
     try pose (X := validTy H wfΔ vσ) ;
     block H
-  | [H : termValidity _ _ _ _ _ _ |- _] =>
+  | [H : termValidity _ _ _ _ _ _ _ |- _] =>
     let X := fresh "R" H in
     try pose (X := validTm H wfΔ vσ) ;
     block H
-  | [H : typeEqValidity _ _ _ _ _ _ |- _] =>
+  | [H : typeEqValidity _ _ _ _ _ _ _ |- _] =>
     let X := fresh "R" H in
     try pose (X := validTyEq H wfΔ vσ) ;
     block H
-  | [H : termEqValidity _ _ _ _ _ _ _ |- _] =>
+  | [H : termEqValidity _ _ _ _ _ _ _ _ |- _] =>
     let X := fresh "R" H in
     try pose (X := validTmEq H wfΔ vσ) ;
     block H
@@ -324,11 +326,11 @@ Ltac instValid vσ :=
 
 Ltac instValidExt vσ' vσσ' :=
   repeat lazymatch goal with
-  | [H : typeValidity _ _ _ _ |- _] =>
+  | [H : typeValidity _ _ _ _ _ |- _] =>
     let X := fresh "RE" H in
     try pose (X := validTyExt H _ _ vσ' vσσ') ;
     block H
-  | [H : termValidity _ _ _ _ _ _ |- _] =>
+  | [H : termValidity _ _ _ _ _ _ _ |- _] =>
     let X := fresh "RE" H in
     try pose (X := validTmExt H _ _ vσ' vσσ') ;
     block H
